src/examples/matmul-tile-f32/Kuiper.MatMulTileF32.Kernel.fsti
@@ -47,7 +47,7 @@ let kpost (rows shared columns: nat)
   I.gpu_pts_to_matrix rows shared ga1 nthr s1
   ** I.gpu_pts_to_matrix shared columns ga2 nthr s2
   ** gpu_pts_to_array1 r tid
-  // ** (exists* s. gpu_pts_to_array_slice r tid (tid+1) s)
+  // ** (exists* s. gpu_pts_to_slice r tid (tid+1) s)
 
 let permute (rows_tile columns_tile bdim: pos)
 : GTot (permutation (i: nat { 0 <= i /\ i < rows_tile * columns_tile * bdim * bdim }))
