src/lib/kuiper/Kuiper.Array.fsti
@@ -14,7 +14,7 @@ module SZ = FStar.SizeT
 
 val gpu_array (a:Type u#0) (sz:nat) : Type u#0
 
-val gpu_pts_to_array_slice
+val gpu_pts_to_slice
   (#a:Type u#0)
   (#sz:nat)
   (x:gpu_array a sz)
@@ -23,6 +23,7 @@ val gpu_pts_to_array_slice
   (v : seq a)
 : slprop
 
+[@@pulse_unfold]
 let gpu_pts_to_array
   (#a:Type u#0)
   (#sz:nat)
@@ -31,7 +32,7 @@ let gpu_pts_to_array
   (v : seq a)
 : slprop
 =
-  gpu_pts_to_array_slice x #f 0 sz v
+  gpu_pts_to_slice x #f 0 sz v
 
 val gpu_pts_to_slice_ref
   (#a:Type u#0)
@@ -41,8 +42,8 @@ val gpu_pts_to_slice_ref
   (i:nat) (j:nat)
   (#v : seq a)
   : stt_ghost unit emp_inames
-      (gpu_pts_to_array_slice x #f i j v)
-      (fun _ -> gpu_pts_to_array_slice x #f i j v **
+      (gpu_pts_to_slice x #f i j v)
+      (fun _ -> gpu_pts_to_slice x #f i j v **
                 pure (i <= j /\ j <= sz /\ Seq.length v == (j-i)
                             /\ SZ.fits (Seq.length v)
                 ))
@@ -86,9 +87,9 @@ fn gpu_array_read
   (#f:perm)
   (idx : SZ.t {i <= SZ.v idx /\ SZ.v idx < j})
   (#s : erased (seq a))
-  requires gpu ** gpu_pts_to_array_slice #a #sz r #f i j s
+  requires gpu ** gpu_pts_to_slice #a #sz r #f i j s
   returns  x:a
-  ensures  gpu ** gpu_pts_to_array_slice #a #sz r #f i j s **
+  ensures  gpu ** gpu_pts_to_slice #a #sz r #f i j s **
             pure (i <= j /\ j <= sz /\ Seq.length s == (j-i) /\
                   x == Seq.index s (SZ.v idx - i))
 
@@ -102,9 +103,9 @@ fn gpu_array_write
   (idx : SZ.t{i <= SZ.v idx /\ SZ.v idx < j})
   (v : a)
   (#s : erased (seq a))
-  requires gpu ** gpu_pts_to_array_slice #a #sz r #1.0R i j s
+  requires gpu ** gpu_pts_to_slice #a #sz r #1.0R i j s
   ensures  gpu **
-            (exists* (s':seq a). gpu_pts_to_array_slice #a #sz r #1.0R i j s' **
+            (exists* (s':seq a). gpu_pts_to_slice #a #sz r #1.0R i j s' **
               pure (i <= j /\ j <= sz /\ Seq.length s == (j-i) /\
                     s' == Seq.upd s (SZ.v idx - i) v))
 
@@ -150,6 +151,8 @@ fn gpu_memcpy_device_to_host
     gpu_pts_to_array src_garr #1.0R gv **
     pure (Seq.length gv == reveal sz)
 
+(* Not making this unfold as it appears under bigstars. Maybe
+pulse should only do weak unfolding. *)
 let gpu_pts_to_array1
   (#a:Type0)
   (#sz:nat)
@@ -157,7 +160,7 @@ let gpu_pts_to_array1
   (#[exact (`1.0R)] f : perm)
   (i:nat)
 : slprop =
-  exists* s. gpu_pts_to_array_slice arr i (i+1) s
+  exists* s. gpu_pts_to_slice arr i (i+1) s
 
 val gpu_array_slice_1
   (#[exact (`0)] uid: int) (#a:Type u#0)
@@ -169,7 +172,7 @@ val gpu_array_slice_1
     unit
     emp_inames
     (gpu_pts_to_array arr #f v)
-    (fun _ -> bigstar #uid 0 sz (fun i -> gpu_pts_to_array_slice arr #f i (i+1) (Seq.cons (Seq.index v i) Seq.empty)))
+    (fun _ -> bigstar #uid 0 sz (fun i -> gpu_pts_to_slice arr #f i (i+1) (Seq.cons (Seq.index v i) Seq.empty)))
 
 val gpu_array_unslice_1
   (#uid: int) (#a:Type u#0)
@@ -180,7 +183,7 @@ val gpu_array_unslice_1
 : stt_ghost
     unit
     emp_inames
-    (bigstar #uid 0 sz (fun i -> gpu_pts_to_array_slice arr #f i (i+1) (Seq.cons (Seq.index v i) Seq.empty)))
+    (bigstar #uid 0 sz (fun i -> gpu_pts_to_slice arr #f i (i+1) (Seq.cons (Seq.index v i) Seq.empty)))
     (fun _ -> gpu_pts_to_array arr #f v)
 
 val gpu_array_slice_1_underspec
@@ -214,8 +217,8 @@ val gpu_slice_concat
   (#s1 #s2: erased (seq a))
   (i n m:nat)
   : stt_ghost unit emp_inames
-      (gpu_pts_to_array_slice arr #f i n s1 ** gpu_pts_to_array_slice arr #f n m s2)
-      (fun _ -> gpu_pts_to_array_slice arr #f i m (Seq.append s1 s2))
+      (gpu_pts_to_slice arr #f i n s1 ** gpu_pts_to_slice arr #f n m s2)
+      (fun _ -> gpu_pts_to_slice arr #f i m (Seq.append s1 s2))
 
 ghost
 fn gpu_slice_slice_1_underspec
@@ -226,8 +229,8 @@ fn gpu_slice_slice_1_underspec
   (#v : erased (seq a))
   (i n:nat)
   (m: nat { i <= m /\ m <= n })
-  requires gpu_pts_to_array_slice arr #f i n v
-  ensures bigstar #uid 0 (m - i) (fun x -> gpu_pts_to_array1 arr #f (x + i)) ** gpu_pts_to_array_slice arr #f m n v
+  requires gpu_pts_to_slice arr #f i n v
+  ensures bigstar #uid 0 (m - i) (fun x -> gpu_pts_to_array1 arr #f (x + i)) ** gpu_pts_to_slice arr #f m n v
 
 ghost
 fn gpu_slice_unslice_1_underspec
@@ -237,8 +240,8 @@ fn gpu_slice_unslice_1_underspec
   (#f : perm)
   (i n:nat)
   (m: nat { i <= m /\ m <= n })
-  requires bigstar #uid 0 (m - i) (fun x -> gpu_pts_to_array1 arr #f (x + i)) ** (exists* v. gpu_pts_to_array_slice arr #f m n v)
-  ensures exists* v. gpu_pts_to_array_slice arr #f i n v
+  requires bigstar #uid 0 (m - i) (fun x -> gpu_pts_to_array1 arr #f (x + i)) ** (exists* v. gpu_pts_to_slice arr #f m n v)
+  ensures exists* v. gpu_pts_to_slice arr #f i n v
 
 ghost
 fn gpu_slice_empty_elim
@@ -246,7 +249,7 @@ fn gpu_slice_empty_elim
   (arr : gpu_array a sz)
   (#f : perm)
   (i : nat)
-  requires exists* v. gpu_pts_to_array_slice arr #f i i v
+  requires exists* v. gpu_pts_to_slice arr #f i i v
   ensures  emp
 
 ghost
@@ -258,8 +261,8 @@ fn gpu_slice_share
   (#v : erased (seq a))
   (m n:nat)
   (k: nat { k > 0 })
-  requires gpu_pts_to_array_slice arr #f m n v
-  ensures bigstar #uid 0 k (fun x -> gpu_pts_to_array_slice arr #(f /. Real.of_int k) m n v)
+  requires gpu_pts_to_slice arr #f m n v
+  ensures bigstar #uid 0 k (fun x -> gpu_pts_to_slice arr #(f /. Real.of_int k) m n v)
 
 ghost
 fn gpu_slice_gather
@@ -270,8 +273,8 @@ fn gpu_slice_gather
   (#v : erased (seq a))
   (m n:nat)
   (k: nat { k > 0 })
-  requires bigstar #uid 0 k (fun x -> gpu_pts_to_array_slice arr #(f /. Real.of_int k) m n v)
-  ensures gpu_pts_to_array_slice arr #f m n v
+  requires bigstar #uid 0 k (fun x -> gpu_pts_to_slice arr #(f /. Real.of_int k) m n v)
+  ensures gpu_pts_to_slice arr #f m n v
 
 ghost
 fn gpu_slice_share_underspec
@@ -281,8 +284,8 @@ fn gpu_slice_share_underspec
   (#f : perm)
   (m n:nat)
   (k: nat { k > 0 })
-  requires exists* v. gpu_pts_to_array_slice arr #f m n v
-  ensures bigstar #uid 0 k (fun x -> exists* v. gpu_pts_to_array_slice arr #(f /. Real.of_int k) m n v)
+  requires exists* v. gpu_pts_to_slice arr #f m n v
+  ensures bigstar #uid 0 k (fun x -> exists* v. gpu_pts_to_slice arr #(f /. Real.of_int k) m n v)
 
 ghost
 fn gpu_slice_gather_underspec
@@ -292,5 +295,5 @@ fn gpu_slice_gather_underspec
   (#f : perm)
   (m n:nat)
   (k: nat { k > 0 })
-  requires bigstar #uid 0 k (fun x -> exists* v. gpu_pts_to_array_slice arr #(f /. Real.of_int k) m n v)
-  ensures exists* v. gpu_pts_to_array_slice arr #f m n v
+  requires bigstar #uid 0 k (fun x -> exists* v. gpu_pts_to_slice arr #(f /. Real.of_int k) m n v)
+  ensures exists* v. gpu_pts_to_slice arr #f m n v
